Working more on the simulation proof

theories/overlay/lang.v
@@ -1060,11 +1060,6 @@ Section opsem.
            fill_item_val, fill_item_no_val_inj, head_ctx_step_val.
   Qed.
 
-  Lemma overlay_lang_mixin': LanguageMixin of_val to_val prim_step.
-  Proof.
-    constructor; eauto using to_of_val, of_to_val, val_stuck.
-  Qed.
-
   Definition is_atomic (e : expr) : Prop :=
     match e with
     | Instr _ => True
@@ -1090,7 +1085,6 @@ End opsem.
 Canonical Structure overlay_ectxi_lang `{MachineParameters} := EctxiLanguage overlay_lang_mixin.
 Canonical Structure overlay_ectx_lang `{MachineParameters} := EctxLanguageOfEctxi overlay_ectxi_lang.
 Canonical Structure overlay_lang `{MachineParameters} := LanguageOfEctx overlay_ectx_lang.
-Canonical Structure overlay_lang' `{MachineParameters} := Language overlay_lang_mixin'.
 
 Hint Extern 20 (PureExec _ _ _) => progress simpl : typeclass_instances.
 
@@ -1181,7 +1175,7 @@ Qed.
 
 Definition overlay_component: Type := component nat _ _ overlay.base.Word.
 
-Definition initial_state `{MachineParameters} (b_stk e_stk: Addr) (c: overlay_component): cfg overlay_lang' :=
+Definition initial_state `{MachineParameters} (b_stk e_stk: Addr) (c: overlay_component): cfg overlay_lang :=
   match c with
   | Lib _ _ _ _ pre_comp => ([Seq (Instr Executable)], (∅, ∅, ∅, [])) (* dummy value *)
   | Main _ _ _ _ (ms, _, _) c_main => ([Seq (Instr Executable)], (<[r_stk := inr (Stk 0 URWLX b_stk e_stk b_stk)]> (<[PC := c_main]> (gset_to_gmap (inl 0%Z) (list_to_set all_registers))), ms, ∅, []))
